Integrate optimised decrypt in EverCrypt

providers/evercrypt/fst/EverCrypt.AEAD.fst
@@ -358,10 +358,10 @@ let encrypt #a s iv ad ad_len plain plain_len cipher tag =
         Success
 
 inline_for_extraction noextract
-let aes_gcm_decrypt (a:aes_gcm_alg): GCMdecrypt_stdcalls.gcm_decrypt_st (vale_alg_of_alg a) =
+let aes_gcm_decrypt (a:aes_gcm_alg): GCMdecryptOpt_stdcalls.decrypt_opt_stdcall_st (vale_alg_of_alg a) =
   match a with
-  | AES128_GCM -> GCMdecrypt_stdcalls.gcm128_decrypt_stdcall
-  | AES256_GCM -> GCMdecrypt_stdcalls.gcm256_decrypt_stdcall
+  | AES128_GCM -> GCMdecryptOpt_stdcalls.gcm128_decrypt_opt_stdcall
+  | AES256_GCM -> GCMdecryptOpt256_stdcalls.gcm256_decrypt_opt_stdcall
 
 #set-options "--z3rlimit 200"
 inline_for_extraction noextract
@@ -385,6 +385,9 @@ fun s iv ad ad_len cipher cipher_len tag dst ->
       // just allocate a temporary on the stack and blit.
       let tmp_keys = B.alloca 0uy (key_offset a) in
       MB.blit ek 0ul tmp_keys 0ul (key_offset a);
+
+      let hkeys_b = B.alloca 0uy 128ul in
+      MB.blit ek (key_offset a) hkeys_b 0ul 128ul;      
 
       // The iv is modified by Vale, which the API does not allow. Hence
       // we allocate a temporary buffer and blit the contents of the iv
@@ -421,7 +424,32 @@ fun s iv ad ad_len cipher cipher_len tag dst ->
       assert_norm (4096 * (pow2 20 - 1) < Words_s.pow2_32);
       assert_norm (4096 * (pow2 20 - 1 - 16) < Words_s.pow2_32);
 
+
       let h0 = get() in
+
+      // There is no SMTPat on le_bytes_to_seq_quad32_to_bytes and the converse,
+      // so we need an explicit lemma
+      let lemma_hkeys_reqs () : Lemma
+        (let k = G.reveal kv in
+        let k_nat = Words.Seq_s.seq_uint8_to_seq_nat8 k in
+        let k_w = Words.Seq_s.seq_nat8_to_seq_nat32_LE k_nat in
+        OptPublic.hkeys_reqs_pub
+          (Types_s.le_bytes_to_seq_quad32 (Words.Seq_s.seq_uint8_to_seq_nat8 (B.as_seq h0 hkeys_b)))
+          (Types_s.reverse_bytes_quad32 (AES_s.aes_encrypt_LE (vale_alg_of_alg a) k_w (Words_s.Mkfour 0 0 0 0))))
+        = let k = G.reveal kv in
+          let k_nat = Words.Seq_s.seq_uint8_to_seq_nat8 k in
+          let k_w = Words.Seq_s.seq_nat8_to_seq_nat32_LE k_nat in
+          let hkeys_quad = OptPublic.get_hkeys_reqs (Types_s.reverse_bytes_quad32 (
+            AES_s.aes_encrypt_LE (vale_alg_of_alg a) k_w (Words_s.Mkfour 0 0 0 0))) in
+          let hkeys = Words.Seq_s.seq_nat8_to_seq_uint8 (Types_s.le_seq_quad32_to_bytes hkeys_quad) in
+          assert (Seq.equal (B.as_seq h0 hkeys_b) hkeys);
+          calc (==) {
+            Types_s.le_bytes_to_seq_quad32 (Words.Seq_s.seq_uint8_to_seq_nat8 hkeys);
+            (==) { Arch.Types.le_bytes_to_seq_quad32_to_bytes hkeys_quad }
+            hkeys_quad;
+          }
+
+      in lemma_hkeys_reqs ();
 
       let r = aes_gcm_decrypt a
         (let k = G.reveal kv in
@@ -434,7 +462,8 @@ fun s iv ad ad_len cipher cipher_len tag dst ->
         tmp_iv
         dst
         tag
-        tmp_keys in
+        tmp_keys 
+        hkeys_b in
 
       let h1 = get() in
 
